txn-data-consistency/EP+_Sorted.thy
@@ -1,0 +1,104 @@
+section \<open>EP+ Event System for well-sorted executions\<close>
+
+theory "EP+_Sorted"
+  imports "EP+"
+begin
+
+\<comment> \<open>Updated Events\<close>
+
+definition read_done_G_s where
+  "read_done_G_s cl kv_map sn u'' s \<equiv>
+    read_done_G cl kv_map sn s \<and>
+    u'' = view_of (cts_order s) (get_view s cl)"
+
+definition read_done_s :: "cl_id \<Rightarrow> (key \<rightharpoonup> 'v) \<Rightarrow> sqn \<Rightarrow> view \<Rightarrow> ('v, 'm) global_conf_scheme \<Rightarrow> ('v, 'm) global_conf_scheme \<Rightarrow> bool" where
+  "read_done_s cl kv_map sn u'' s s' \<equiv>
+    read_done_G_s cl kv_map sn u'' s \<and>
+    s' = read_done_U cl kv_map s"
+
+definition write_commit_G_s where
+  "write_commit_G_s cl kv_map cts sn u'' s \<equiv>
+    write_commit_G cl kv_map cts sn s \<and>
+    u'' = view_of (cts_order s) (get_view s cl) \<and>
+    (\<forall>k \<in> dom kv_map. \<forall>t \<in> set (cts_order s k). (cts, cl) > unique_ts (wtxn_cts s) t)"
+
+definition write_commit_s :: "cl_id \<Rightarrow> (key \<rightharpoonup> 'v) \<Rightarrow> tstmp \<Rightarrow> sqn \<Rightarrow> view \<Rightarrow> ('v, 'm) global_conf_scheme \<Rightarrow> ('v, 'm) global_conf_scheme \<Rightarrow> bool" where
+  "write_commit_s cl kv_map cts sn u'' s s' \<equiv>
+    write_commit_G_s cl kv_map cts sn u'' s \<and> 
+    s' = write_commit_U cl kv_map cts s"
+
+
+subsection \<open>The Event System\<close>
+
+fun state_trans :: "('v, 'm) global_conf_scheme \<Rightarrow> 'v ev \<Rightarrow> ('v, 'm) global_conf_scheme \<Rightarrow> bool" where
+  "state_trans s (RInvoke cl keys)          s' \<longleftrightarrow> read_invoke cl keys s s'" |
+  "state_trans s (Read cl k v t rts rlst)   s' \<longleftrightarrow> read cl k v t rts rlst s s'" |
+  "state_trans s (RDone cl kv_map sn u'')   s' \<longleftrightarrow> read_done_s cl kv_map sn u'' s s'" |
+  "state_trans s (WInvoke cl kv_map)        s' \<longleftrightarrow> write_invoke cl kv_map s s'" |
+  "state_trans s (WCommit cl kv_map cts sn u'') s' \<longleftrightarrow> write_commit_s cl kv_map cts sn u'' s s'" |
+  "state_trans s (WDone cl kv_map)          s' \<longleftrightarrow> write_done cl kv_map s s'" |
+  "state_trans s (RegR svr t t_wr rts)      s' \<longleftrightarrow> register_read svr t t_wr rts s s'" |
+  "state_trans s (PrepW svr t v)            s' \<longleftrightarrow> prepare_write svr t v s s'" |
+  "state_trans s (CommitW svr t v cts)      s' \<longleftrightarrow> commit_write svr t v cts s s'" |
+  "state_trans s Skip2 s' \<longleftrightarrow> s' = s"
+
+definition tps :: "('v ev, 'v global_conf) ES" where
+  "tps \<equiv> \<lparr>
+    init = (=) state_init,
+    trans = state_trans
+  \<rparr>"
+
+lemmas tps_trans_top_defs = 
+  read_invoke_def read_def read_done_s_def write_invoke_def write_commit_s_def
+  write_done_def register_read_def prepare_write_def commit_write_def
+
+lemmas tps_trans_GU_defs = 
+  read_invoke_G_def read_invoke_U_def
+  read_G_def read_U_def
+  read_done_G_def read_done_U_def read_done_G_s_def
+  write_invoke_G_def write_invoke_U_def
+  write_commit_G_def write_commit_U_def write_commit_G_s_def
+  write_done_G_def write_done_U_def
+  register_read_G_def register_read_U_def
+  prepare_write_G_def prepare_write_U_def
+  commit_write_G_def commit_write_U_def
+
+lemmas tps_trans_defs = tps_trans_top_defs tps_trans_GU_defs
+
+lemmas tps_trans_all_defs = tps_trans_defs ext_corder_def
+
+lemmas tps_defs = tps_def state_init_def
+
+lemma tps_trans [simp]: "trans tps = state_trans" by (simp add: tps_def)
+
+
+subsection \<open>Simulation function\<close>
+
+term "Set.filter (is_done s) rs"
+
+definition txn_to_vers :: "('v, 'm) global_conf_scheme \<Rightarrow> key \<Rightarrow> txid \<Rightarrow> 'v version" where
+  "txn_to_vers s k = (\<lambda>t. case svr_state (svrs s k) t of
+    Prep ts v \<Rightarrow> \<lparr>v_value = v, v_writer = t, v_readerset = {}\<rparr> |
+    Commit cts ts lst v rs \<Rightarrow> \<lparr>v_value = v, v_writer = t, v_readerset = {t. \<exists>rts rlst. (t, rts, rlst) \<in> rs \<and> is_done s t}\<rparr>)"
+
+definition kvs_of_s :: "'v global_conf \<Rightarrow> 'v kv_store" where
+  "kvs_of_s s \<equiv> (\<lambda>k. map (txn_to_vers s k) (cts_order s k))"
+
+lemmas kvs_of_s_defs = kvs_of_s_def txn_to_vers_def
+
+definition views_of_s :: "'v global_conf \<Rightarrow> (cl_id \<Rightarrow> view)" where
+  "views_of_s s = (\<lambda>cl. view_of (cts_order s) (get_view s cl))"
+
+definition sim :: "'v global_conf \<Rightarrow> 'v config" where         
+  "sim s = (kvs_of_s s, views_of_s s)"
+
+lemmas sim_defs = sim_def kvs_of_s_defs views_of_s_def
+
+subsection \<open>Mediator function\<close>
+
+fun med :: "'v ev \<Rightarrow> 'v label" where
+  "med (RDone cl kv_map sn u'') = ET cl sn u'' (read_only_fp kv_map)" |
+  "med (WCommit cl kv_map _ sn u'') = ET cl sn u'' (write_only_fp kv_map)" |
+  "med _ = ETSkip"
+
+end
